Distance $= \csc\theta + \cot\theta$

Circumference $= k\csc\theta$

Let $c = \frac{k}{2\pi}$ be the radius of the bottleneck.

scale $= \frac{c\csc\theta}{r}$

%$E = G = \frac{r^2}{c^2\csc^2\theta}, F = 0$

$\frac{d\theta}{dr} = \frac{c\csc\theta}{r}$

By Wolfram Alpha,

$\theta = \cos^{-1}(k_1 - c\log r)$

$\cos\theta = k_1 - c\log r$

$\cos\theta - k_1 = -c\log r$

$\frac{k_1 - \cos\theta}{c} = \log r$

$r = e^\frac{k_1 - \cos\theta}{c}$

For $k_1 = 0$:

$\theta = \cos^{-1}(-c\log r)$

$r = e^-\frac{\cos\theta}{c}$

Scale $= \frac{c^2\csc\theta}{\cos\theta}$

$= \frac{c^2}{\sin\theta\cos\theta}$

Or in terms of $r$,

Scale $= \frac{c\csc\theta}{r}$

$= \frac{c}{r\sin\theta}$

$= \frac{c}{r\sqrt{1-\cos^2\theta}}$

$= \frac{c}{r\sqrt{1-c^2 \log^2 r}}$

\ignore{
$F = 0$

$E = G = \frac{r^2(1-c^2 \log^2 r)}{c^2}$

$= \frac{r^2}{c^2} - \log^2 r$

$= \frac{x^2+y^2}{c^2} - \frac{1}{4}\log^2(x^2+y^2)$

$E_u = G_u = \frac{2x}{c^2} - 2\frac{1}{4}\log(x^2+y^2)\frac{1}{2x}$

$= \frac{2x}{c^2} - \frac{1}{4x}\log(x^2+y^2)$

$E_v = G_v = \frac{2y}{c^2} - \frac{1}{4y}\log(x^2+y^2)$

$K = -\frac{1}{2\sqrt{EG}}\left(\frac{\partial}{\partial u}\frac{G_u}{\sqrt{EG}} + \frac{\partial}{\partial v}\frac{E_v}{\sqrt{EG}}\right)$

$= -\frac{1}{2E}\left(\frac{\partial}{\partial u}\frac{E_u}{E} + \frac{\partial}{\partial v}\frac{E_v}{E}\right)$

%$\frac{\partial}{\partial u}\frac{E_u}{E} = \frac{\partial}{\partial u} \frac{\frac{2x}{c^2} - 2\frac{1}{4}\log(x^2+y^2)\frac{1}{2x}}{\frac{x^2+y^2}{c^2} - \frac{1}{4}\log^2(x^2+y^2)}$

$= -\frac{1}{2E}\left(\frac{E E_{uu} - E_u^2}{E^2} + \frac{E E_{vv} - E_v^2}{E^2}\right)$

$= \frac{E_u^2 + E_v^2}{2E^3} - \frac{E_{uu}+E_{uv}}{2E^2}$

%$= -\frac{1}{2E^3}\left(E E_{uu} - E_u^2 + E E_{vv} - E_v^2\right)$

$E_{uu} = \frac{\partial}{\partial u} \frac{2x}{c^2} - \frac{1}{4x}\log(x^2+y^2)$

$= \frac{2}{c^2} - \frac{1}{4x}\frac{2x}{x^2+y^2} + \frac{1}{4x^2}\log(x^2+y^2)$

$= \frac{2}{c^2} - \frac{1}{2(x^2+y^2)} + \frac{\log(x^2+y^2)}{4x^2}$

$E_{vv} = \frac{2}{c^2} - \frac{1}{2(x^2+y^2)} + \frac{\log(x^2+y^2)}{4y^2}$
}